
\begin{tcolorbox}[colback=green!5!white,colframe=green!75!black,title=\textbf{\textsc{Newton}-type
		methods}]
	Only consider active inequality constraints $\rightarrow$ only equality-conditions\\
	Iteration:
	\begin{flalign*}
		\begin{bmatrix}
			w_{k+1} \\ \lambda_{k+1}
		\end{bmatrix}
		&=
		\begin{bmatrix}
			w_k \\ 0
		\end{bmatrix}
		-
		\underbrace{
			\begin{bmatrix}
				B_k & \nabla_w g(w_k) \\
				\nabla_w g(w_k)^\top & 0\\
			\end{bmatrix}^{-1}
		}_\text{inverse\ KKT-Matrix}
		\begin{bmatrix}
			\nabla_w f(w_k) \\
			g(w_k)
		\end{bmatrix}\\
		&=
		\begin{bmatrix}
			w_k \\ \lambda_k
		\end{bmatrix}
		- 
		\begin{bmatrix}
			B_k & \nabla_w g(w_k) \\
			\nabla_w g(w_k)^\top & 0\\
		\end{bmatrix}^{-1}
		\begin{bmatrix}
			\nabla_w L(w_k, \lambda) \\
			g(w)
		\end{bmatrix}\\
	\end{flalign*}
	Exact \textsc{Newton}: $B_k = \nabla_w^2\mathcal{L}(w_k,\lambda_k)$, \textit{quadratic convergence}\\
	\textsc{Gauss-Newton}:  $f(w) = \frac{1}{2} \| R(w) \|_2^2$:$B_k = \sum_{i=1}^{n_R} \nabla_w R_i(w_k) \nabla_w R_i(w_k)^\top$\\ \textit{linear convergence}\\
	\textsc{BFGS} Quasi-Newton: $B_{k+1} = - \frac{B_k s_k s_k^\top B_k}{s_k^\top B_k s_k} + \frac{y_k y_k^\top}{s_k y_k^\top}$\\
	secant condition $B_{k+1} s_k = y_k$, step $s_k = w_{k+1} - w_k$, gradient step: $y_k = \nabla_w \mathcal{L}(w_{k+1}, \lambda_{k+1}) - \nabla_w \mathcal{L}(w_{k}, \lambda_{\mathbf{k+1}})$, \textit{super linear convergence}
\end{tcolorbox}