
\begin{tcolorbox}[colback=lime!5!white,%
  colframe=lime!75!black,%
  title=\textbf{Sequential and Simultaneous approach}]
  \textbf{Basic problem formulation}
  \begin{align*}
    \begin{array}{|rl|}\hline
    \min_w &F(w) \\
    \mathrm{s.t.}\quad & G(w) \\ \hline
    \end{array}, %% dirty hack, I know
    F(w)&:= \sum^{N-1}_{k=0} L(x_k,u_k) + E(x_N) \\
    G(w)&:=
          \left[
          \begin{array}{c}
            f(x_0,u_0)-x_1 \\
            f(x_1,u_1)-x_2 \\
            \dots \\
            f(x_{N-1},u_{N-1})-x_N \\
            r(x_0,x_N)
          \end{array}
          \right]
  \end{align*}
  \textbf{KKT for simultaneous approach}
  \begin{flalign*}
    \nabla_{x_0}\mathcal{L}(w,\lambda) &= \nabla_{x_0}L(x_0,u_0) +
    \nabla_{x_0}f(x_0,u_0)\lambda_1 + \nabla_{x_0}r(x_0, x_N)\lambda_r &=
    0 \\
    \nabla_{x_k}\mathcal{L}(w,\lambda) &= \nabla_{x_k}L(x_k,u_k) +
    \nabla_{x_k}f(x_k,u_k)\cdot \lambda_{k+1} - \lambda_k  &= 0 \\
    \nabla_{x_N}\mathcal{L}(w,\lambda) &= \nabla_{x_N}E(x_N) + \nabla_{x_N}r(x_N)\cdot
    \lambda_r - \lambda_N  &= 0 \\
    \nabla_{u_k}\mathcal{L}(w,\lambda) &= \nabla_{u_k}L(x_k, u_k) + \nabla_{u_k}f(x_k,u_k)\cdot \lambda_{k+1} &= 0 \\
  \end{flalign*}
  \textbf{KKT for sequential approach}
  \begin{flalign*}
    x_0 &= \bar{x}_0 \\
    x_{k+1} &= f(x_k, u_k) \\
    \lambda_N &= \nabla_{x_N}E(x_N) \\
    \lambda_k &= \nabla_{x_k}L(x_k, u_k) + \nabla_{x_k}f(x_k, u_k) \lambda_{k+1}
    \\
   0 &= \nabla_{u_k}L(x_k,u_k) + \nabla_{u_k}f(x_k, u_k) \lambda_{k+1}
 \end{flalign*}\\
 
  \textbf{Sparse QP} One SQP step solves the problem:
  \begin{align*}
    \min_{\Delta w}\quad &\nabla F(w)^T \Delta w + 0.5 \Delta w^T \nabla^2_w\mathcal{L}(w,\lambda, \mu)\Delta w \\
    \mathrm{s.t.}\quad & G(w) + \nabla G(w)^T \Delta w = 0, \\
    & H(w) + \nabla H(w)^T\Delta w \le 0
  \end{align*}
  Now:
  \begin{flalign*}
    Q_k := \nabla^2_{w_k}\mathcal{L}(w,\lambda, \mu),\quad g_k:=\nabla(w)L(w_k),\quad g_N:=\nabla(x_N)E(x_N) \\
    a := f(x_k, u_k) - x_{k+1}, \quad A_k:=\nabla_{x_k}f(x_k,u_k), \quad B_k:=
    \nabla_{u_k} f(x_k, u_k) \\
    r:=\sum^{N-1}_{k=0}r_k(x_k,u_k) + r_N(x_N),\quad
    R_k:=\nabla_{x_k,u_k}r_k(x_k,u_k) \\
    (\mathrm{Gleicher\ Scheiss\ mit\ } h_k,h_N, \mathrm{usw.}),\quad
    R_N:=\nabla_{x_N}r_N
  \end{flalign*}
  Then:
  \begin{flalign*}
    \min_{\Delta w}\quad & 0.5\left(\sum^{N-1}_{k=0} \Delta w_k^T Q_k w_k + \Delta x_N^T Q_N
    \Delta x_N\right) + \sum^N_{k=0}\Delta w_k^T g_k + \Delta x_N g_N \\
    \mathrm{s.t.}\quad& a_k + A_k\Delta x_k + B_k \Delta u_k - \Delta x_{k+1} =
    0 \\
    & r + \sum^{N-1}_{k=0} R_k\Delta w + R_N\Delta x_N = 0 \\
    & h_k + H_k \Delta w \le 0 \\
    & h_N + H_N\Delta x_N \le 0
  \end{flalign*}
  \textbf{Condensing an SQP:} System:
  \begin{align*}
    \Delta x_{k+1}=a_k + A_k x_{k} + B_k u_k
  \end{align*}
  split up $\Delta w \rightarrow \Delta
  w_\mathrm{dep}, \Delta w_\mathrm{indep}$
  \begin{align*}
    \left[
    \begin{array}{c}
      \Delta x_1 \\ \dots \\ \Delta x_N
    \end{array}
    \right] = v + M 
    \left[
    \begin{array}{c}
      \Delta x_0 \\ \Delta u_1 \\ \dots \\ \Delta u_{N-1}
    \end{array}
    \right],\quad v_1=a_0, v_{k+1} = a_k + A_k v_k
  \end{align*}
  $M$ is lower triangular, bc. $\Delta x_j$ indep. of $u_k$ if $k>j$
  
\end{tcolorbox}
%%% Local Variables:
%%% mode: latex
%%% TeX-master: "../HelpSheet"
%%% TeX-engine: xetex
%%% End:
